ew.fst
@@ -1,0 +1,161 @@
+module Ew
+
+open FStar.List.Tot
+open Library
+
+type o =
+    | Enable
+    | Disable
+
+type s = nat * bool
+       
+val app_op : s -> o -> s
+let app_op (c,f) o = 
+  match o with
+  | Enable -> (c + 1, true)
+  | Disable -> (c, false)
+
+instance ew : datatype s o = {
+   Library.apply_op = app_op
+}
+
+val vis : o -> o -> Tot bool
+let vis a b = admit()
+
+val visib : l:list o -> o1:o -> o2:o -> bool
+let visib l o1 o2 = mem o1 l && mem o2 l && vis o1 o2
+
+val sum : list o -> nat
+let rec sum l =
+    match l with
+    |[] -> 0
+    |(Enable)::xs -> 1 + sum xs
+    |(Disable)::xs -> sum xs
+    
+val sim : s0:s
+        -> tr:list o
+        -> s1:s 
+        -> Tot bool           
+let sim s0 tr s1 = 
+        let c = fst s0 + sum tr in
+        let f = if ((for_all (fun e -> (existsb (fun d -> (d = Disable) && visib tr e d)) tr) (filter (fun e -> (e = Enable)) tr)) ||
+                    (for_all (fun e -> (e = Disable)) tr)) then false else true in
+        s1 = (c,f)
+
+val union : l:list o 
+          -> a:list o
+          -> b:list o
+          -> list o          
+let rec union l a b = 
+    match l,a,b with
+    |[],[],[] -> []
+    |x::xs, _, _ -> x::(union xs a b)
+    |[],x::xs,_ -> x::(union [] xs b)
+    |[],[],_ -> b
+
+assume val axiom : l:list o -> a:list o -> b:list o
+                 -> Lemma (ensures (forall o1 o2. visib (union l a b) o1 o2 ==> visib l o1 o2 \/ visib a o1 o2 \/ visib b o1 o2)) [SMTPat (union l a b)]
+    
+val merge_flag : l:s 
+               -> a:s{fst a >= fst l}
+               -> b:s{fst b >= fst l}
+               -> bool
+let merge_flag l a b =
+      let lc = fst l in
+      let ac = fst a in
+      let bc = fst b in
+      let af = snd a in
+      let bf = snd b in
+      if af && bf then true
+      else if not af && not bf then false
+      else if af then ac - lc > 0
+      else bc - lc > 0
+
+val merge : init:s
+          -> ltr:list o
+          -> l:s
+          -> atr:list o 
+          -> a:s 
+          -> btr:list o 
+          -> b:s 
+          -> Pure s (requires (sim init ltr l /\ sim l atr a /\ sim l btr b) /\ 
+                   (forall o1 o2 o3. mem o1 ltr /\ mem o2 atr /\ mem o3 btr ==> visib (union ltr atr btr) o1 o2 /\ visib (union ltr atr btr) o1 o3) /\ 
+                   (forall o1 o2. (visib ltr o1 o2 ==> visib atr o1 o2 /\ visib btr o1 o2)))
+                   (ensures (fun res -> true))
+let merge init ltr l atr a btr b = 
+    let c = fst a + fst b - fst l in
+    let f = merge_flag l a b in
+      c, f
+
+
+val lemma1 : l:list o
+           -> a:list o
+           -> b:list o
+           -> Lemma (ensures (forall ele. mem ele (union l a b) <==> mem ele l \/ mem ele a \/ mem ele b) /\ (sum (union l a b) = sum l + sum a + sum b)) (decreases %[l;a;b])           
+let rec lemma1 l a b = 
+  match l,a,b with
+  |[],[],[] -> ()
+  |x::xs, _, _ -> lemma1 xs a b
+  |[],x::xs,_ -> lemma1 [] xs b
+  |[],[],x::xs -> lemma1 [] [] xs
+
+
+(************* This part is to check whether the counter values are the same - BEGIN ********************************************)
+val sim1 : s0:s
+         -> tr:list o
+         -> s1:s 
+         -> Tot bool           
+let sim1 s0 tr s1 = 
+         let c = fst s0 + sum tr in
+         let f = if ((for_all (fun e -> (existsb (fun d -> (d = Disable) && visib tr e d)) tr) (filter (fun e -> (e = Enable)) tr)) ||
+                     (for_all (fun e -> (e = Disable)) tr)) then false else true in
+         fst s1 = c
+
+val prop1 : init:s
+          -> ltr: list o
+          -> l:s 
+          -> atr:list o 
+          -> a:s 
+          -> btr:list o
+          -> b:s 
+          -> Lemma (ensures ((sim init ltr l /\ sim l atr a /\ sim l btr b) /\ 
+                  (forall o1 o2 o3. mem o1 ltr /\ mem o2 atr /\ mem o3 btr ==> visib (union ltr atr btr) o1 o2 /\ visib (union ltr atr btr) o1 o3) /\ 
+                  (forall o1 o2. (visib ltr o1 o2 ==> visib atr o1 o2 /\ visib btr o1 o2)) ==> 
+                  (sim1 init (union ltr atr btr) (merge init ltr l atr a btr b))))                    
+let prop1 init ltr l atr a btr b = 
+    lemma1 ltr atr btr; ()
+
+(************* This part is to check whether the counter values are the same - END ********************************************)
+    
+val prop : init:s
+         -> ltr: list o
+         -> l:s 
+         -> atr:list o 
+         -> a:s 
+         -> btr:list o
+         -> b:s 
+         -> Lemma (ensures (sim init ltr l /\ sim l atr a /\ sim l btr b) /\ 
+                 (forall o1 o2 o3. mem o1 ltr /\ mem o2 atr /\ mem o3 btr ==> visib (union ltr atr btr) o1 o2 /\ visib (union ltr atr btr) o1 o3) /\ 
+                 (forall o1 o2. (visib ltr o1 o2 ==> visib atr o1 o2 /\ visib btr o1 o2)) ==> 
+                 (sim init (union ltr atr btr) (merge init ltr l atr a btr b)))
+                 
+let prop init ltr l atr a btr b = 
+  lemma1 ltr atr btr; admit()
+
+val convergence : init:s 
+                -> tr:list o
+                -> a:s 
+                -> b:s 
+                -> Lemma (requires (sim init tr a /\ sim init tr b))
+                        (ensures (a = b))
+let convergence inir tr a b = ()
+
+
+instance _ : mrdt s o ew = {
+    Library.sim = sim;
+    Library.visib = visib;
+    Library.union = union;
+    Library.merge = merge;
+    Library.prop = prop;
+    Library.convergence = convergence
+  }
